\documentclass[../thesis.tex]{subfiles}
\begin{document}

\chapter{The Ising model as an open quantum system}

\section{Solution of the transverse Ising model}

We consider the Hamiltonian
\begin{equation}
  \ham
  = -J\sum_{i \in \ZZ_N} \opr{S}_i^x\opr{S}_{i+1}^x
  - \Gamma\sum_{i \in \ZZ_N} \opr{S}_i^z,
\end{equation}
which we nondimensionalize as
\begin{equation}
  \frac{4}{J}\ham
  = -\sum_{i \in \ZZ_N} \pauli_i^x\pauli_{i+1}^x
  + \lambda\sum_{i \in \ZZ_N} \pauli_i^z
  \label{eq:transham}
\end{equation}
\todo[inline]{Note that $\ham$ does not have $4/J$ below. Fix this and change
$\lambda$ (Striff) to $-\alpha$.}
for the periodic transverse Ising chain with $N$ spins. We notice that the
operators
\begin{equation}
  \pauli_i^\pm
  = \frac{\pauli_i^x \pm \im\pauli_i^y}{2}
  \label{eq:paulipm}
\end{equation}
satisfy
\begin{equation}
  \pauli_i^z
  = 2\pauli_i^+\pauli_i^- - \idopr
\end{equation}
and have commutators
\begin{align}
  \comm{\pauli_i^+}{\pauli_j^-}
  &= \frac{1}{4}\comm{\pauli_i^x + \im\pauli_i^y}{\pauli_j^x - \im\pauli_j^y} \\
  &= \frac{1}{4} \qty(%
  \comm{\pauli_i^x}{\pauli_j^x} + \comm{\pauli_i^y}{\pauli_j^y}
  + \im\comm{\pauli_i^y}{\pauli_j^x}
  - \im\comm{\pauli_i^x}{\pauli_j^y}
  ) \\
  &= \delta_{ij}\pauli_i^z.
\end{align}
Thus their anticommutators are
\begin{align}
  \acomm{\pauli_i^+}{\pauli_j^-}
  &= 2\pauli_i^+\pauli_j^- - \comm{\pauli_i^+}{\pauli_j^-} \\
  &= 2\pauli_i^+\pauli_j^- - \delta_{ij}\pauli_i^z \\
  &= \delta_{ij}\idopr + 2\pauli_i^+\pauli_j^- (1 - \delta_{ij}).
\end{align}
It could be helpful to think of the $\pauli_i^\pm$ as fermion creation and
annihilation operators, but they do not anticommute at different sites.

How might we construct operators that satisfy the fermionic canonical
anticommutation relations (CARs) from the Pauli operators? Suppose we have such
operators $\opr{c}_i$. Given a tuple $\tq{n} = {\qty(n_i)}_{i\in\ZZ_N}$, we have the
corresponding states
\begin{equation}
  \ket{\tq{n}}
  = \prod_{i\in\ZZ_N} {\qty(\opr{c}_i^\dag)}^{n_i} \ket{\tq{0}},
\end{equation}
where $\ket{\tq{0}}$ denotes the vacuum state. It then follows that
\begin{align}
  \opr{c}_i\ket{\tq{n}}
  &= -n_i {(-1)}^{n_{<i}}\ket{\tq{n}_{i \leftarrow 0}}
  \label{eq:car-action} \\
  \opr{c}_i^\dag\ket{\tq{n}}
  &= -(1 - n_i){(-1)}^{n_{<i}}\ket{\tq{n}_{i \leftarrow 1}},
\end{align}
where $\tq{n}_{i \leftarrow m} = \tq{n}$ with $n_i = m$ and $n_{<i} = \sum_{j <
i} n_j$.

Thus the number operator is
\begin{align}
  \opr{c}_i^\dag \opr{c}_i \ket{\tq{n}}
  &= (1-0){(-1)}^{n_{<i}} n_i{(-1)}^{n_{<i}} \ket{\tq{n}_{i \leftarrow 1}} \\
  &= n_i\ket{\tq{n}}.
\end{align}

This leads us to consider
\begin{align}
  \opr{c}_i
  = -\qty(\prod_{j<i} -\pauli_j^z) \pauli_i^-
\end{align}
acting on the states
\begin{equation}
  \ket{\tq{n}}
  = \prod_{i \in \ZZ_N} {\qty(\pauli_i^+)}^{n_i} \ket{\tq{0}},
\end{equation}
where $\ket{\tq{0}} = \ket{\uparrow}^{\tp N}$ is the state with all $z$-spins
up, or all zero qubits. This gives the same result as \cref{eq:car-action}, so
the $\opr{c}_i$ satisfy the CARs. This process of mapping spin-1/2 sites to
non-local fermions is known as the \term{Jordan-Wigner transformation}. We may
then compute that the inverse transformations are
\begin{align}
  \pauli_i^+\pauli_i^-
  &= \opr{c}_i^\dag\opr{c}_i
  \label{eq:paulipm} \\
  \pauli_i^z
  &= 2\opr{c}_i^\dag\opr{c}_i - \idopr
  \label{eq:pauliz} \\
  \pauli_i^x
  &= -\qty(\prod_{j<i} \qty(\idopr - 2\opr{c}_j^\dag\opr{c}_j))
  \qty(\opr{c}_i^\dag + \opr{c}_i)
  \label{eq:paulix} \\
  \pauli_i^y
  &= \im\qty(\prod_{j<i} \qty(\idopr - 2\opr{c}_j^\dag\opr{c}_j))
  \qty(\opr{c}_i^\dag - \opr{c}_i).
  \label{eq:pauliy}
\end{align}
While $\pauli_i^x$ remains complicated, the product $\pauli_i^x\pauli_{i+1}^x$
does not. For $i < N-1$,
\begin{align}
  \pauli_i^x \pauli_{i+1}^x
  &= \qty(\prod_{j<i} \qty(2\opr{c}_j^\dag\opr{c}_j - \idopr))
  \qty(\opr{c}_i^\dag + \opr{c}_i)
  \qty(\prod_{j<i+1} \qty(2\opr{c}_j^\dag\opr{c}_j - \idopr))
  \qty(\opr{c}_{i+1}^\dag + \opr{c}_{i+1}) \\
  &= \qty(\opr{c}_i^\dag + \opr{c}_i)
  \qty(\idopr - 2\opr{c}_i^\dag\opr{c}_i)
  \qty(\opr{c}_{i+1}^\dag + \opr{c}_{i+1}) \\
  &= \qty(\opr{c}_i^\dag - \opr{c}_i) \qty(\opr{c}_{i+1}^\dag + \opr{c}_{i+1}),
  \label{eq:paulixx}
\end{align}
and for $i = N-1$,
\begin{equation}
  \pauli_{N-1}^x \pauli_0^x
  = \qty(\prod_{j < N-1} \qty(2\opr{c}_j^\dag\opr{c}_j - \idopr))
  \qty(\opr{c}_{N-1}^\dag + \opr{c}_{N-1})
  \qty(\opr{c}_0^\dag + \opr{c}_0).
\end{equation}

We may now perform the Jordan-Wigner transformation of \cref{eq:transham} to
obtain\todo[inline]{Check boundary term to Pfeuty~(2.4). Why can it be neglected
for large $N$?}
\begin{align}
  \ham
  &= \sum_i \qty(\opr{c}_i - \opr{c}_i^\dag) \qty(\opr{c}_{i+1}^\dag + \opr{c}_{i+1})
  + \lambda\sum_i 2\opr{c}_i^\dag\opr{c}_i
  - \lambda N \idopr \\
  &- \qty(\idopr - \prod_{j < N-1}\qty(2\opr{c}_j^\dag \opr{c}_j - \idopr))
  \qty(\opr{c}_{N-1} - \opr{c}_{N-1}^\dag) \qty(\opr{c}_0^\dag + \opr{c}_0)
  \label{eq:cham}
\end{align}
We now Fourier transform with
\begin{subequations}
\begin{align}
  \opr{c}_i
  &= \frac{1}{\sqrt{N}}\sum_k e^{\im ki} \opr{C}_k
  \label{eq:fourierc} \\
  \opr{C}_k
  &= \frac{1}{\sqrt{N}}\sum_i e^{-\im ki} \opr{c}_i
  \label{eq:fourierC} \\
  \shortintertext{and}
  \opr{c}_i^\dag
  &= \frac{1}{\sqrt{N}}\sum_k e^{-\im ki} \opr{C}_k^\dag
  \label{eq:fourierct} \\
  \opr{C}_k^\dag
  &= \frac{1}{\sqrt{N}}\sum_i e^{\im ki} \opr{c}_i^\dag
  \label{eq:fourierCt}.
\end{align}\label{eq:fourier}
\end{subequations}
\begin{proof}
  \begin{align}
    \opr{c}_0
    &= \frac{1}{\sqrt{N}}\sum_k \opr{C}_k \\
    \opr{c}_N
    &= \frac{1}{\sqrt{N}}\sum_k e^{\im kN} \opr{C}_k.
  \end{align}
  We then must require that
  \begin{equation}
    kN
    \equiv 0 \pmod{2\pi}
  \end{equation}
  \begin{equation}
    k
    = \frac{2\pi n}{N} - \frac{N - [\text{$N$ odd}]}{N}\pi \qc
    n \in \ZZ_N.
    \label{eq:fourierk}
  \end{equation}
  For $N$ odd, what is $C_{\pi}$?
  \begin{align}
    % \opr{C}_\pi
    \opr{C}_{\pi}
    &= \frac{1}{\sqrt{N}} \sum_i e^{-\im \pi i} \opr{c}_i.
  \end{align}
  Since $e^{-\im\pi i} = e^{\im\pi i}$, $\opr{C}_\pi = \opr{C}_{-\pi}$.
\end{proof}
\begin{proof}
  Consider $N$ fermionic operators $\opr{c}_i$ and a $N \times N$ unitary matrix
  $\mq{U}$. We may change bases with
  \begin{equation}
    \opr{C}_k^\dag
    = \sum_i U_{ik} \opr{c}_i^\dag.
  \end{equation}
  Then
  \begin{align}
    \acomm{\opr{C}_k}{\opr{C}_{k'}^\dag}
    &= \sum_{ij} U_{ik}^*U_{jk'} \acomm{\opr{c}_i}{\opr{c}_j^\dag} \\
    &= \sum_i U_{ik}^*U_{ik'} \\
    &= {\qty(\mq{U}^\dag\mq{U})}_{kk'} \\
    &= \delta_{kk'},
  \end{align}
  and similar for the other fermionic (anti)-commutation relations.
\end{proof}
\begin{proof}
  For the Fourier transform,
  \begin{equation}
    F_{ik}
    = \frac{1}{\sqrt{N}} e^{\im ki}.
  \end{equation}
  We may then confirm that
  \begin{align}
    {\qty(\mq{F}^\dag\mq{F})}_{kk'}
    &= \sum_i \frac{1}{N} e^{\im (k' - k)i} \\
    &= \delta_{kk'}.
  \end{align}
  Thus the Fourier transform is unitary.
\end{proof}
Now since
\begin{equation}
  \frac{1}{N}\sum_{i\in\ZZ_N} e^{\im(k' - k) i}
  = \delta_{kk'},
\end{equation}
and also
\begin{align}
  \opr{C}_{-k}
  &= \opr{C}_k^* \\
  &= \frac{1}{\sqrt{N}} \sum_i e^{-\im (-k)i} \opr{c}_i \\
  &= \frac{1}{N}\sum_{ik'} e^{\im (k' + k)i} \opr{C}_{k'},
\end{align}
we have that
\begin{align}
  \sum_i \opr{c}_i^\dag\opr{c}_i
  &= \frac{1}{N}\sum_{ikk'} e^{\im (k' - k)i}
  \opr{C}_k^\dag \opr{C}_{k'} \\
  &= \sum_k \opr{C}_k^\dag \opr{C}_k,
  \\
  \sum_i \qty(\opr{c}_i^\dag\opr{c}_{i+1} + \opr{c}_{i+1}^\dag\opr{c}_i)
  &= \frac{1}{N}\sum_{ikk'} e^{\im (k' - k)i} \qty(%
  e^{\im k'} + e^{-\im k} 
  ) \opr{C}_k^\dag \opr{C}_{k'} \\
  &= \sum_k 2 \cos k\; \opr{C}_k^\dag \opr{C}_k,
  \\
  \sum_i \qty(\opr{c}_{i+1}\opr{c}_i + \opr{c}_i^\dag\opr{c}_{i+1}^\dag)
  &= \frac{1}{N}\sum_{ikk'} \qty(%
  e^{\im (k' + k)i} e^{\im k} \opr{C}_{k}\opr{C}_{k'}
  + e^{-\im (k' + k)i} e^{-\im k'} \opr{C}_{k}^\dag\opr{C}_{k'}^\dag
  ) \\
  &= \sum_k \qty(%
  e^{-\im k} \opr{C}_{-k} \opr{C}_k
  + e^{\im k} \opr{C}_k^\dag \opr{C}_{-k}^\dag
  ).
\end{align}
Thus \cref{eq:cham} is now
\begin{align}
  \ham
  &= -\sum_k 2 \cos k\; \opr{C}_k^\dag \opr{C}_k
  + \sum_k \qty(%
  e^{-\im k} \opr{C}_{-k} \opr{C}_k
  + e^{\im k} \opr{C}_k^\dag \opr{C}_{-k}^\dag
  )
  + \sum_k 2\lambda\opr{C}_k^\dag\opr{C}_k
  - \lambda N \idopr
  \\
  &= \sum_k \qty(\lambda - \cos k)
  \qty(%
  \opr{C}_k^\dag \opr{C}_k
  + \opr{C}_{-k}^\dag \opr{C}_{-k}
  )
  + \sum_k \im\sin k
  \qty(%
  \opr{C}_{-k}\opr{C}_k
  - \opr{C}_k^\dag\opr{C}_{-k}^\dag
  )
  - \lambda N \idopr
  \\
  &= \sum_k \qty(\lambda - \cos k)
  \qty(%
  \opr{C}_k^\dag \opr{C}_k
  - \opr{C}_{-k} \opr{C}_{-k}^\dag
  )
  + \sum_k \im\sin k
  \qty(%
  \opr{C}_{-k}\opr{C}_k
  - \opr{C}_k^\dag\opr{C}_{-k}^\dag
  ) \\
  &= \sum_k \vq{v}_k^\dag \mq{H}_k \vq{v}_k,
  \label{eq:Cham} \\
  \shortintertext{where}
  \mq{H}_k
  &= \bmqty{%
  \lambda - \cos k & -\im\sin k \\
  \im\sin k & \cos k - \lambda
  }, \\
  \vq{v}_k
  &= \bmqty{\opr{C}_k \\ \opr{C}_{-k}^\dag},
\end{align}
and we have used that
\begin{equation}
  \sum_k \cos k = 0.
\end{equation}
Since the $\mq{H}_k$ are Hermitian, they may be diagonalized by a unitary
transformation of the $\vq{v}_k$. The $\mq{H}_k$ are traceless, so they have the
eigenvalues
\begin{align}
  E_k^\pm
  &= \pm\sqrt{-\det\mq{H}_k} \\
  &= \pm\sqrt{\lambda^2 - 2\lambda\cos k + \cos^2 k + \sin^2 k} \\
  &= \pm\sqrt{\lambda^2 - 2\lambda\cos k + 1}.
\end{align}
The eigenvectors are then
\begin{equation}
  \vq{q}_k^\pm
  = \bmqty{%
    -\im\sin k \\
    E_k^\pm - (\lambda - \cos k)
  },
\end{equation}
except if $k = 0$ or $-\pi$, in which case
\begin{align}
  \vq{q}_k^-
  &= \bmqty{1 \\ 0}
  \qand
  \vq{q}_k^+
  = \bmqty{0 \\ 1}.
\end{align}
The $k = -\pi$ case does not appear if $N$ is odd. If also $\lambda =
-1$, then $\mq{H}_{-\pi} = \mq{0}$.
To construct the unitary
transformation, we must normalize the $\vq{q}_k^\pm$. We find that
\begin{align}
  \norm{\vq{q}_k^\pm}^2
  &= {\qty(E_k^\pm - (\lambda - \cos k))}^2 + \sin^2 k \\
  &= {\qty(E_k^\pm)}^2 + \lambda^2 + \cos^2 k - 2\lambda\cos k - 2E_k^\pm(\lambda - \cos k) + 1 - \cos^2 k \\
  &= 2E_k^\pm \qty(E_k^\pm - (\lambda - \cos k)).
\end{align}
Now
\begin{align}
  \frac{{\qty(\vq{q}_k^\pm)}_1}{\norm{\vq{q}_k^\pm}}
  &= \frac{-\im\sin k}{\sqrt{2E_k^\pm \qty(E_k^\pm - (\lambda - \cos k))}} \\
  &= \frac{-\im\sin k}{\sqrt{2\abs{E_k^\pm} \qty(\abs{E_k^\pm} \mp (\lambda - \cos k))}}
  \\
  \shortintertext{and}
  %
  \frac{{\qty(\vq{q}_k^\pm)}_2}{\norm{\vq{q}_k^\pm}}
  &= \pm\sqrt{\frac{E_k^\pm - (\lambda - \cos k)}{2E_k^\pm}} \\
  &= \pm\sqrt{\frac{\abs{E_k^\pm} \mp (\lambda - \cos k)}{2\abs{E_k^\pm}}}
\end{align}
\begin{equation}
  \mq{U}_k^\dag
  = \bmqty{%
    {\qty(\hat{\vq{q}}_k^-)}^\dag \\
    {\qty(\hat{\vq{q}}_k^+)}^\dag
  }.
\end{equation}
Then with $E_k = \abs{E_k^\pm}$,
\begin{equation}
  \opr{\eta}_k^\pm
  = \frac{\im\sin k}{\sqrt{2E_k\qty(E_k \pm (\cos k - \lambda))}}
  \opr{C}_k
  \pm \sqrt{\frac{E_k \pm (\cos k - \lambda)}{2E_k}}
  \opr{C}^\dag_{-k}
  \label{eq:etas}
\end{equation}
so that
\begin{align}
  \acomm{{\qty(\opr{\eta}_k^\pm)}^\dag}{\opr{\eta}_k^\pm}
  &= \frac{\sin^2 k}{2E_k\qty(E_k \pm (\cos k - \lambda))} \idopr
  + \frac{E_k \pm (\cos k - \lambda)}{2E_k} \idopr \\
  &= \idopr
  \\
  \begin{split}
  \acomm{{\qty(\opr{\eta}_k^\pm)}^\dag}{\opr{\eta}_k^\mp}
  &= \frac{\sin^2 k}{2E_k
    \sqrt{E_k \pm (\cos k - \lambda)}
  \sqrt{E_k \mp (\cos k - \lambda)}} \idopr \\
  &- \frac{\sqrt{E_k \pm (\cos k - \lambda)}\sqrt{E_k \mp (\cos k - \lambda)}}{%
  2 E_k} \idopr
  \end{split}
  \\
  &= \zopr.
\end{align}
Note that \cref{eq:etas} is consistent with the edge cases in the limits $k \to
-\pi$ and $k \to 0$. If also $\lambda = -1$, then we impose that
$\opr{\eta}_{-\pi} = \opr{C}_\pi^\dag$, which is the same as if $\lambda \ne
-1$.

\Cref{eq:Cham} becomes
\begin{equation}
  \ham
  = \sum_k E_k^+{\qty(\opr{\eta}_k^+)}^\dag\opr{\eta}_k^+
  + \sum_k E_k^-{\qty(\opr{\eta}_k^-)}^\dag\opr{\eta}_k^-.
  \label{eq:etasham}
\end{equation}
Since
\begin{equation}
  {\qty(\opr{\eta}_{-k}^-)}^\dag
  = \opr{\eta}_k^+
  \eqqcolon \opr{\eta}_k
\end{equation}
and $E_{-k}^\pm = E_k^\pm$, we may reduce \cref{eq:etasham} to
\begin{align}
  \ham
  &= \sum_k E_k\opr{\eta}_k^\dag \opr{\eta}_k
  - \sum_k E_k\qty(\idopr - \opr{\eta}_k^\dag \opr{\eta}_k)
  \\
  &= \sum_k 2E_k\opr{\eta}_k^\dag\opr{\eta}_k
  - \idopr\sum_k E_k.
  \label{eq:etaham}
\end{align}

The unitary transformation of the $\opr{C}_{\pm k}$ to obtain $\opr{\eta}_k^\pm$
is an instance of a fermionic \term{Bogoliubov transformation}:
\begin{subequations}
  \begin{align}
    \opr{C}_k
  &= u\opr{f}_k + v\opr{g}_k^\dag \\
  \shortintertext{and}
  \opr{C}_{-k}
  &= -v\opr{f}_k^\dag + u\opr{g}_k.
  \end{align}\label{eq:bogoliubov}
\end{subequations}
For these transformations to preserve the CARs,
\begin{align}
  \acomm{\opr{C}_k^\dag}{\opr{C}_k}
  &= \abs{u}^2 \acomm{\opr{f}_k^\dag}{\opr{f}_k}
  + \abs{v}^2 \acomm{\opr{g}_k}{\opr{g}_k^\dag}
  + u^* v \acomm{\opr{f}_k^\dag}{\opr{g}_k^\dag}
  + v^* u \acomm{\opr{g}_k}{\opr{f}_k} \\
  &= \qty(\abs{u}^2 + \abs{v}^2) \idopr,
\end{align}
so we must have
\begin{equation}
  \abs{u}^2 + \abs{v}^2 = 1.
\end{equation}
We may choose
% \begin{subequations}
  \begin{align}
    u &= e^{\im\phi_1}\cos\theta \\
    v &= e^{\im\phi_2}\sin\theta
  \end{align}\label{eq:uv-param}
% \end{subequations}
for real angles $\phi_1$, $\phi_2$, and $\theta$.

It remains to perform the inverse transformations to obtain the $\pauli_i^x$ in
terms of the $\opr{\eta}_k^\pm$. Shift of perspective: Instead of decomposing
the Hilbert space as the tensor product of spin operators, we decompose
it as the tensor product of fermionic operators, where the fermionic operators
are restricted to their subspaces in order to form an orthonormal basis for the
Liouville space. We may then recover $\pauli_i^x$ by the corresponding
isomorphism of Liouville spaces. We choose
\begin{equation}
  \opr{c}
  \qc
  \opr{c}^\dag
  \qc
  \opr{c}^\dag \opr{c},
  \qand
  \opr{c} \opr{c}^\dag
\end{equation}
as our basis, since they are both orthonormal and eigenoperators of
$\opr{c}^\dag \opr{c} \angle$ with respective eigenvalues
\[
  -1 \qc 1 \qc 2, \qand 0.
\]

% Notebooks
% \notebook{transverse-ising}
% \notebook{jump-operators}

\notebook{sym-two-spin-jumps}

\clearpage
\section{Two-spin degenerate jump operators}

(Divided by $2$.)

For $\omega = 0$:
\begin{align}
2\pauli_1^x
\\
2\pauli_2^x
\end{align}

For $\omega = -4$:
\begin{align}
\pauli_1^y - \im \pauli_1^z \pauli_2^x
\\
\im \pauli_1^y \pauli_2^x + \pauli_1^z
\\
-\im \pauli_1^x \pauli_2^z + \pauli_2^y
\\
\im \pauli_1^x \pauli_2^y + \pauli_2^z
\end{align}

For $\omega = 4$:
\begin{align}
\pauli_1^y + \im \pauli_1^z \pauli_2^x
\\
-\im \pauli_1^y \pauli_2^x + \pauli_1^z
\\
\im \pauli_1^x \pauli_2^z + \pauli_2^y
\\
-\im \pauli_1^x \pauli_2^y + \pauli_2^z
\end{align}


\section{Two-spin nondegenerate jump operators}

\todo[inline]{%
  Simplify further: better operators and collecting noncommutative terms as
  usual.
}

\begin{sidewaysfigure}[!htb]
  \tiny
  \begin{align}
    \input{../notebooks/nondegen-jumps.tex}
  \end{align}
  \caption{The jump operators for the nondegenerate case ($g \ne 0$).}\label{fig:two-spin-nondegen-jumps}
\end{sidewaysfigure}

\begin{sidewaysfigure}[!htb]
  \tiny
  \begin{align}
    \input{../notebooks/degen-jumps.tex}
  \end{align}
  \caption{The jump operators for the degenerate case ($g = 0$).}\label{fig:two-spin-degen-jumps}
\end{sidewaysfigure}

See \cref{fig:two-spin-nondegen-jumps,fig:two-spin-degen-jumps}.

Let $d = \sqrt{g^2 + 1}$.

For $\omega = -4 d$:
\begin{align}
-\sqrt{2} g \pauli_1^x \pauli_2^x + \sqrt{2} g \pauli_1^y \pauli_2^y + \sqrt{2} \im d \pauli_1^x \pauli_2^y + \sqrt{2} \im d \pauli_1^y \pauli_2^x + \sqrt{2} \pauli_1^z + \sqrt{2} \pauli_2^z
\end{align}

For $\omega = -2 d - 2$:
{\tiny
\begin{align}
-\im g^2 \pauli_1^x - \im g^2 \pauli_1^x \pauli_2^z + g^2 \pauli_1^z \pauli_2^y + g^2 \pauli_2^y - g d \pauli_1^y - g d \pauli_1^y \pauli_2^z + \im g d \pauli_1^z \pauli_2^x + \im g d \pauli_2^x - g \pauli_1^y + \im g \pauli_1^z \pauli_2^x - \im d \pauli_1^x \pauli_2^z + d \pauli_2^y - \im \pauli_1^x \pauli_2^z + \pauli_2^y
\\
g^2 \pauli_1^x + g^2 \pauli_1^x \pauli_2^z + \im g^2 \pauli_1^z \pauli_2^y + \im g^2 \pauli_2^y - \im g d \pauli_1^y - \im g d \pauli_1^y \pauli_2^z - g d \pauli_1^z \pauli_2^x - g d \pauli_2^x + \im g \pauli_1^y \pauli_2^z + g \pauli_2^x - d \pauli_1^x - \im d \pauli_1^z \pauli_2^y + \pauli_1^x + \im \pauli_1^z \pauli_2^y
\\
\im g^2 \pauli_1^y + \im g^2 \pauli_1^y \pauli_2^z + g^2 \pauli_1^z \pauli_2^x + g^2 \pauli_2^x - g d \pauli_1^x - g d \pauli_1^x \pauli_2^z - \im g d \pauli_1^z \pauli_2^y - \im g d \pauli_2^y + g \pauli_1^x + \im g \pauli_1^z \pauli_2^y - \im d \pauli_1^y \pauli_2^z - d \pauli_2^x + \im \pauli_1^y \pauli_2^z + \pauli_2^x
\\
g^2 \pauli_1^y + g^2 \pauli_1^y \pauli_2^z - \im g^2 \pauli_1^z \pauli_2^x - \im g^2 \pauli_2^x + \im g d \pauli_1^x + \im g d \pauli_1^x \pauli_2^z - g d \pauli_1^z \pauli_2^y - g d \pauli_2^y + \im g \pauli_1^x \pauli_2^z - g \pauli_2^y + d \pauli_1^y - \im d \pauli_1^z \pauli_2^x + \pauli_1^y - \im \pauli_1^z \pauli_2^x
\end{align}
}

For $\omega = 2 d + 2$:
{\tiny
\begin{align}
\im g^2 \pauli_1^x + \im g^2 \pauli_1^x \pauli_2^z + g^2 \pauli_1^z \pauli_2^y + g^2 \pauli_2^y - g d \pauli_1^y - g d \pauli_1^y \pauli_2^z - \im g d \pauli_1^z \pauli_2^x - \im g d \pauli_2^x - g \pauli_1^y - \im g \pauli_1^z \pauli_2^x + \im d \pauli_1^x \pauli_2^z + d \pauli_2^y + \im \pauli_1^x \pauli_2^z + \pauli_2^y
\\
-\im g^2 \pauli_1^y - \im g^2 \pauli_1^y \pauli_2^z + g^2 \pauli_1^z \pauli_2^x + g^2 \pauli_2^x - g d \pauli_1^x - g d \pauli_1^x \pauli_2^z + \im g d \pauli_1^z \pauli_2^y + \im g d \pauli_2^y + g \pauli_1^x - \im g \pauli_1^z \pauli_2^y + \im d \pauli_1^y \pauli_2^z - d \pauli_2^x - \im \pauli_1^y \pauli_2^z + \pauli_2^x
\\
g^2 \pauli_1^y + g^2 \pauli_1^y \pauli_2^z + \im g^2 \pauli_1^z \pauli_2^x + \im g^2 \pauli_2^x - \im g d \pauli_1^x - \im g d \pauli_1^x \pauli_2^z - g d \pauli_1^z \pauli_2^y - g d \pauli_2^y - \im g \pauli_1^x \pauli_2^z - g \pauli_2^y + d \pauli_1^y + \im d \pauli_1^z \pauli_2^x + \pauli_1^y + \im \pauli_1^z \pauli_2^x
\\
g^2 \pauli_1^x + g^2 \pauli_1^x \pauli_2^z - \im g^2 \pauli_1^z \pauli_2^y - \im g^2 \pauli_2^y + \im g d \pauli_1^y + \im g d \pauli_1^y \pauli_2^z - g d \pauli_1^z \pauli_2^x - g d \pauli_2^x - \im g \pauli_1^y \pauli_2^z + g \pauli_2^x - d \pauli_1^x + \im d \pauli_1^z \pauli_2^y + \pauli_1^x - \im \pauli_1^z \pauli_2^y
\end{align}
}

For $\omega = 0$:
{\tiny
\begin{align}
4 \sqrt{2} g^4 + 4 \sqrt{2} g^4 \pauli_1^z + 4 \sqrt{2} g^4 \pauli_1^z \pauli_2^z + 4 \sqrt{2} g^4 \pauli_2^z + 4 \sqrt{2} g^3 \pauli_1^x \pauli_2^x - 4 \sqrt{2} g^3 \pauli_1^y \pauli_2^y + 4 \sqrt{2} g^2 + 2 \sqrt{2} g^2 \pauli_1^z + 4 \sqrt{2} g^2 \pauli_1^z \pauli_2^z + 2 \sqrt{2} g^2 \pauli_2^z + 2 \sqrt{2} g \pauli_1^x \pauli_2^x - 2 \sqrt{2} g \pauli_1^y \pauli_2^y
\end{align}
}

For $\omega = 2 - 2 d$:
{\tiny
\begin{align}
\im g^2 \pauli_1^x + \im g^2 \pauli_1^x \pauli_2^z + g^2 \pauli_1^z \pauli_2^y + g^2 \pauli_2^y + g d \pauli_1^y + g d \pauli_1^y \pauli_2^z + \im g d \pauli_1^z \pauli_2^x + \im g d \pauli_2^x - g \pauli_1^y - \im g \pauli_1^z \pauli_2^x - \im d \pauli_1^x \pauli_2^z - d \pauli_2^y + \im \pauli_1^x \pauli_2^z + \pauli_2^y
\\
g^2 \pauli_1^y + g^2 \pauli_1^y \pauli_2^z + \im g^2 \pauli_1^z \pauli_2^x + \im g^2 \pauli_2^x + \im g d \pauli_1^x + \im g d \pauli_1^x \pauli_2^z + g d \pauli_1^z \pauli_2^y + g d \pauli_2^y - \im g \pauli_1^x \pauli_2^z - g \pauli_2^y - d \pauli_1^y - \im d \pauli_1^z \pauli_2^x + \pauli_1^y + \im \pauli_1^z \pauli_2^x
\\
g^2 \pauli_1^x + g^2 \pauli_1^x \pauli_2^z - \im g^2 \pauli_1^z \pauli_2^y - \im g^2 \pauli_2^y - \im g d \pauli_1^y - \im g d \pauli_1^y \pauli_2^z + g d \pauli_1^z \pauli_2^x + g d \pauli_2^x - \im g \pauli_1^y \pauli_2^z + g \pauli_2^x + d \pauli_1^x - \im d \pauli_1^z \pauli_2^y + \pauli_1^x - \im \pauli_1^z \pauli_2^y
\\
-\im g^2 \pauli_1^y - \im g^2 \pauli_1^y \pauli_2^z + g^2 \pauli_1^z \pauli_2^x + g^2 \pauli_2^x + g d \pauli_1^x + g d \pauli_1^x \pauli_2^z - \im g d \pauli_1^z \pauli_2^y - \im g d \pauli_2^y + g \pauli_1^x - \im g \pauli_1^z \pauli_2^y - \im d \pauli_1^y \pauli_2^z + d \pauli_2^x - \im \pauli_1^y \pauli_2^z + \pauli_2^x
\end{align}
}

For $\omega = 2 d - 2$:
{\tiny
\begin{align}
g^2 \pauli_1^y + g^2 \pauli_1^y \pauli_2^z - \im g^2 \pauli_1^z \pauli_2^x - \im g^2 \pauli_2^x - \im g d \pauli_1^x - \im g d \pauli_1^x \pauli_2^z + g d \pauli_1^z \pauli_2^y + g d \pauli_2^y + \im g \pauli_1^x \pauli_2^z - g \pauli_2^y - d \pauli_1^y + \im d \pauli_1^z \pauli_2^x + \pauli_1^y - \im \pauli_1^z \pauli_2^x
\\
g^2 \pauli_1^x + g^2 \pauli_1^x \pauli_2^z + \im g^2 \pauli_1^z \pauli_2^y + \im g^2 \pauli_2^y + \im g d \pauli_1^y + \im g d \pauli_1^y \pauli_2^z + g d \pauli_1^z \pauli_2^x + g d \pauli_2^x + \im g \pauli_1^y \pauli_2^z + g \pauli_2^x + d \pauli_1^x + \im d \pauli_1^z \pauli_2^y + \pauli_1^x + \im \pauli_1^z \pauli_2^y
\\
-\im g^2 \pauli_1^x - \im g^2 \pauli_1^x \pauli_2^z + g^2 \pauli_1^z \pauli_2^y + g^2 \pauli_2^y + g d \pauli_1^y + g d \pauli_1^y \pauli_2^z - \im g d \pauli_1^z \pauli_2^x - \im g d \pauli_2^x - g \pauli_1^y + \im g \pauli_1^z \pauli_2^x + \im d \pauli_1^x \pauli_2^z - d \pauli_2^y - \im \pauli_1^x \pauli_2^z + \pauli_2^y
\\
\im g^2 \pauli_1^y + \im g^2 \pauli_1^y \pauli_2^z + g^2 \pauli_1^z \pauli_2^x + g^2 \pauli_2^x + g d \pauli_1^x + g d \pauli_1^x \pauli_2^z + \im g d \pauli_1^z \pauli_2^y + \im g d \pauli_2^y + g \pauli_1^x + \im g \pauli_1^z \pauli_2^y + \im d \pauli_1^y \pauli_2^z + d \pauli_2^x + \im \pauli_1^y \pauli_2^z + \pauli_2^x
\end{align}
}

For $\omega = 4 d$:
\begin{align}
-\sqrt{2} g \pauli_1^x \pauli_2^x + \sqrt{2} g \pauli_1^y \pauli_2^y - \sqrt{2} \im d \pauli_1^x \pauli_2^y - \sqrt{2} \im d \pauli_1^y \pauli_2^x + \sqrt{2} \pauli_1^z + \sqrt{2} \pauli_2^z
\end{align}

For $\omega = 4$:
\begin{align}
-\im \pauli_1^x \pauli_2^y + \im \pauli_1^y \pauli_2^x - \pauli_1^z + \pauli_2^z
\\
\im \pauli_1^x \pauli_2^y - \im \pauli_1^y \pauli_2^x + \pauli_1^z - \pauli_2^z
\end{align}

For $\omega = -4$:
\begin{align}
\im \pauli_1^x \pauli_2^y - \im \pauli_1^y \pauli_2^x - \pauli_1^z + \pauli_2^z
\\
-\im \pauli_1^x \pauli_2^y + \im \pauli_1^y \pauli_2^x + \pauli_1^z - \pauli_2^z
\end{align}

\end{document}

