\documentclass[../thesis.tex]{subfiles}
\begin{document}

\chapter{The generator of a quantum dynamical semigroup}\label{ch:lindblad}

\emph{The contents of this appendix follow~\cite{opensys}.}

Let $\sopr{V}(t)$ for $t \ge 0$ be a family of completely positive and
trace-preserving \textsc{cptp} maps on $\liou(\hilb)$ with the \term{semigroup
property} that
\begin{equation}
  \sopr{V}(t)\sopr{V}(s)
  = \sopr{V}(t + s).
\end{equation}
In the physical context, $\sopr{V}(t)$ is a dynamical map for the reduced
dynamics of a system, and the semigroup property is that the dynamics are
Markovian or memoryless, just like when one coarse-grains to the system time in
the weak-coupling limit.

By analogy to Stone's theorem, we expect that there is a generator $\sopr{L}$ of
the semigroup such that
\begin{equation}
  \sopr{V}(t)
  = e^{\sopr{L} t}.
\end{equation}
We are interested in obtaining a \term{master equation} of the form
\begin{equation}
  \dot{\dop}
  = \sopr{L}\dop.
\end{equation}

We may find $\sopr{L}$ as follows. Since $\sopr{V}(t)$ is \textsc{cptp}, it may
be decomposed with the help of the Kraus representation theorem as
\begin{equation}
  \sopr{V}(t) \dop
  = \sum_i \opr{M}_i(t)\dop\opr{M}_i^\dag(t),
  \label{eq:krausrep}
\end{equation}
where $\sum_i \opr{M}_i^\dag(t) \opr{M}_i = \idopr$. We can express the
$\opr{M}_i$ in terms of an orthonormal complete basis $\{\opr{F}_n\}$ for
$\liou(\hilb)$ as $\opr{M}_i = \sum_n \opr{F}_n
\lprod{\opr{F}_n}{\opr{M}_i}$. Then \cref{eq:krausrep} becomes
\begin{equation}
  \sopr{V}(t) \dop
  = \sum_{mn} c_{mn}(t) \opr{F}_m\dop\opr{F}_n^\dag,
  \label{eq:Fintro}
\end{equation}
where
\begin{equation}
  c_{mn}(t)
  \equiv \sum_i \lprod{\opr{F}_m}{\opr{M}_i(t)}\lprod{\opr{M}_i(t)}{\opr{F}_n}.
  \label{eq:kraus-coeffs}
\end{equation}
For convenience, we may choose $\opr{F}_{d^2} = \idopr / \sqrt{d}$, where $d =
\dim(\hilb)$. With an eye towards simplifying \cref{eq:Vderiv}, we eliminate
the explicit time dependence of \cref{eq:kraus-coeffs} by defining
\begin{equation}
  a_{mn}
  \equiv \lim_{t \to 0^+} \frac{c_{mn}(t) - d\delta_{d^2 d^2}}{t}
  \label{eq:limcoeffs}
\end{equation}
and introduce the sum of Kraus operators
\begin{align}
  \opr{F}
  &= \frac{1}{\sqrt{d}}\sum_{n=1}^{d^2 - 1} a_{n d^2} \opr{F}_n
  \label{eq:kraussum} \\
  &= \frac{\opr{F} + \opr{F}^\dag}{2}
  + \im \frac{\opr{F} - \opr{F}^\dag}{2\im}
  \equiv \opr{G} - \im\ham,
  \label{eq:kraussherm}
\end{align}
where we have decomposed the sum $\opr{F}$ into Hermitian and anti-Hermitian
parts. Now we may write the master equation $\dot{\dop} = \liou\dop$ as
\begin{align}
  \dot{\dop}
  &= \lim_{\Delta t \to 0^+} \frac{\sopr{V}(\Delta t)\dop - \dop}{\Delta t} \\
  %
  \begin{split}
  &= \lim_{\Delta t \to 0^+} \Bigg(%
  \frac{c_{d^2 d^2} - d}{d\Delta t} \dop
  + \sum_{m,n=1}^{d^2 - 1}
  \frac{c_{mn}(\Delta t)}{\Delta t}\opr{F}_m \dop \opr{F}_n^\dag \\
  &\hphantom{= \lim_{\Delta t \to 0^+} \Bigg.}
  + \frac{1}{\sqrt{d}} \sum_{n=1}^{d^2 - 1} \qty(%
  \frac{c_{nd^2}(\Delta t)}{\Delta t} \opr{F}_n \dop
  + \frac{c_{d^2 n}(\Delta t)}{\Delta t} \dop \opr{F}_n^\dag)
  \Bigg)
  \end{split}
  \label{eq:Vderiv} \\
  %
  &= \frac{a_{d^2 d^2}}{d} \dop 
  + \opr{F}\dop + \dop\opr{F}^\dag
  + \sum_{m,n=1}^{d^2 - 1} a_{mn} \opr{F}_m \dop \opr{F}_n^\dag \\
  %
  &= \frac{a_{d^2 d^2}}{d} \dop 
  + \acomm{\opr{G}}{\dop}
  - \im\comm{\ham}{\dop}
  + \sum_{m,n=1}^{d^2 - 1} a_{mn} \opr{F}_m \dop \opr{F}_n^\dag \\
  %
  &= \acomm{\opr{G}'}{\dop}
  - \im\comm{\ham}{\dop}
  + \sum_{m,n=1}^{d^2 - 1} a_{mn} \opr{F}_m \dop \opr{F}_n^\dag,
  \label{eq:GHform}
\end{align}
where $\opr{G}' = \opr{G} + \flatfrac{a_{d^2 d^2} \idopr}{d}$. Since
$\sopr{V}(t)$ is trace-preserving, $\tr\dot{\dop} = 0$. Applying this
condition to \cref{eq:GHform} and cycling the trace gives
\begin{equation}
  0
  = \tr\qty(2\opr{G}'\dop
  + \sum_{m,n=1}^{d^2 - 1} a_{mn} \opr{F}_n^\dag \opr{F}_m \dop),
\end{equation}
so $\opr{G}' = -\sum_{m,n=1}^{d^2 - 1} a_{mn} \opr{F}_n^\dag\opr{F}_m / 2$. This
allows us to write \cref{eq:GHform} as
\begin{equation}
  \dot{\dop}
  = -\im\comm{\ham}{\dop}
  + \sum_{m,n=1}^{d^2 - 1} a_{mn}\qty(\opr{F}_m\dop\opr{F}_n^\dag -
  \frac{1}{2}\acomm{\opr{F}_n^\dag \opr{F}_m}{\dop}),
  \label{eq:markovian}
\end{equation}
which is the first form of the \term{Lindblad equation}. This may be simplified
further if we diagonalize the coefficient matrix $\opr{a}$ by applying a unitary
transformation $\opr{u}$ to give $\opr{a} = \opr{u}\opr{Î³}\opr{u}^\dag$, where
the $\qty{\gamma_k}_{k=1}^{d^2 - 1}$ are the non-negative eigenvalues of
$\opr{a}$. This is possible since the coefficient matrix $\opr{c}$ is seen
from \cref{eq:kraus-coeffs} to be Hermitian, and \cref{eq:limcoeffs} then gives
that $\opr{a}$ is Hermitian. We may then express $\opr{F}_{n \neq d^2} =
\sum_{k=1}^{d^2 - 1} \opr{L}_n u_{nk}$ in terms of the \termalt{Lindblad
operators}{Lindblad} or \termalt{jump operator}{jump operators} $\opr{L}_n$ to
find
\begin{equation}
  \dot{\dop}
  = -\im\comm{\ham}{\dop}
  + \sum_{k=1}^{d^2 - 1} \gamma_k \qty(\opr{L}_k\dop\opr{L}_k^\dag -
  \frac{1}{2}\acomm{\opr{L}_k^\dag \opr{L}_k}{\dop}),
  \label{eq:lindblad}
\end{equation}
which is the diagonal form of the Lindblad equation.

It has been proven that that this is the most general generator for a quantum
dynamical semigroup when the system is finite-dimensional~\cite{gks} and when
the system is infinite-dimensional but $\sopr{L}$ is bounded~\cite{lindblad}.
This is not much help, since the Hamiltonians for even simple
infinite-dimensional systems like the harmonic oscillator are unbounded.
Regardless, most examples where $\sopr{L}$ is unbounded may still be cast into
Lindblad form with little or no modification.

\end{document}

